verify/Enumerate62.v
@@ -1,0 +1,272 @@
+Require Import List.
+Require Import Lia.
+From BusyCoq Require Import Individual62.
+From BusyCoq Require Import CTL62.
+From BusyCoq Require Import TC.
+From BusyCoq Require Import Eqb.
+
+Module TC := TC BB62.
+Import TC.
+
+Definition makeTM(a0 a1 b0 b1 c0 c1 d0 d1 e0 e1 f0 f1:option (Sym*dir*Q)):TM :=
+fun '(s,m) =>
+match s,m with
+| A,S0 => a0
+| A,S1 => a1
+| B,S0 => b0
+| B,S1 => b1
+| C,S0 => c0
+| C,S1 => c1
+| D,S0 => d0
+| D,S1 => d1
+| E,S0 => e0
+| E,S1 => e1
+| F,S0 => f0
+| F,S1 => f1
+end.
+
+Definition tm_simpl(tm:TM):TM :=
+makeTM
+(tm (A,S0))
+(tm (A,S1))
+(tm (B,S0))
+(tm (B,S1))
+(tm (C,S0))
+(tm (C,S1))
+(tm (D,S0))
+(tm (D,S1))
+(tm (E,S0))
+(tm (E,S1))
+(tm (F,S0))
+(tm (F,S1)).
+
+Lemma tm_simpl_spec tm:
+  eqv (tm_simpl tm) tm.
+Proof.
+  unfold tm_simpl.
+  eapply perm_eqv with (f:=fun x=>x); eauto.
+  unfold Perm.
+  split; intros q s; destruct q,s; cbn; tauto.
+Qed.
+
+Lemma tm_simpl_spec' tm h:
+  (tm_simpl tm h) = tm h.
+Proof.
+  destruct h as [q s].
+  destruct q,s; reflexivity.
+Qed.
+
+Definition tm_upd(tm:TM)(h:Q*Sym)(y:Sym*dir*Q):TM :=
+  tm_simpl (fun x => if eqb x h then Some y else tm x).
+
+Module TNF_Node.
+Record T := {
+  tm: TM;
+  num_undef_trans: nat;
+  min_unused_state: nat;
+}.
+
+Definition Nat_sum(x:list nat) := List.fold_right Nat.add O x.
+
+Definition get_num_undef_trans(tm:TM) :=
+Nat_sum (List.map (fun q => Nat_sum (List.map (fun s => if tm (q,s) then 0 else 1)%nat all_syms)) all_qs).
+
+Fixpoint In_dec{A}(eq:forall a b:A,{a=b}+{a<>b})(x:A)(ls:list A):{List.In x ls}+{~List.In x ls}.
+Proof.
+  destruct ls as [|h t].
+  - right.
+    intros H.
+    inverts H.
+  - destruct (eq x h).
+    + left. cbn. left. congruence.
+    + destruct (In_dec A eq x t); cbn.
+      * left; tauto.
+      * right. intuition.
+Defined.
+
+Definition WF(x:T):Prop :=
+let (tm,n,m):=x in
+n = get_num_undef_trans tm /\
+match List.skipn m all_qs with
+| nil => True
+| q1::qs =>
+  Perm tm tm (fun q => if In_dec eqb_q q qs then q1 else q)
+end.
+
+Lemma all_qs_nodup: List.NoDup all_qs.
+Proof.
+  repeat econstructor.
+  all:
+  match goal with
+  | |- ~List.In ?x ?ls => pose (In_dec eqb_q x ls) as H;
+    cbn in *;
+    destruct H eqn:E;
+    [ unfold H in E; congruence
+    | apply n ]
+  end.
+Qed.
+
+Definition expand(x:T)(h:Q*Sym):list T.
+Proof.
+  refine (
+  let (tm,n,m):=x in _).
+  refine (_ ++ _)%list.
+  - refine (flat_map (fun s => _) (firstn m all_qs)).
+    refine (flat_map (fun o => _) all_syms).
+    refine (List.map (fun d => _) [L;R]).
+    refine (Build_T (tm_upd tm h (o,d,s)) (Nat.pred n) m).
+  - refine (match skipn m all_qs with
+            | nil => nil
+            | q1::qs => _
+            end).
+    refine (flat_map (fun o => _) all_syms).
+    refine (List.map (fun d => _) [L;R]).
+    refine (Build_T (tm_upd tm h (o,d,q1)) (Nat.pred n) (S m)).
+Defined.
+
+Definition expand'(x:T)(h:Q*Sym):list T :=
+  if eqb x.(num_undef_trans) (S O) then [] else expand x h.
+
+Definition node0 := Build_T (TM_from_str "1RB---_------_------_------_------_------") 11 2.
+
+Definition SearchQueue:Type := (list T)*(list T).
+Open Scope list.
+
+Fixpoint length_tail_0{A}(ls:list A)(n:N):N :=
+match ls with
+| nil => n
+| h::t => length_tail_0 t (N.succ n)
+end.
+
+Definition length_tail{A}(ls:list A):N :=
+  length_tail_0 ls N0.
+
+Definition num_holdout(q:SearchQueue):N :=
+length_tail (snd q).
+
+Definition root_1RB:SearchQueue := ([node0],[]).
+
+Definition get_SQ(q:SearchQueue+SearchQueue):SearchQueue :=
+match q with
+| inl x => x
+| inr x => x
+end.
+
+Definition SearchQueue_upd(f:TM->DecideResult)(q:SearchQueue):SearchQueue+SearchQueue :=
+let (q1,q2):=q in
+match q1 with
+| nil => inr q
+| x::q1' =>
+  inl
+  match f x.(tm) with
+  | Halt h => (expand' x h ++ q1',q2)
+  | NonHalt => (q1',q2)
+  | Unknown => (q1',x::q2)
+  end
+end.
+
+Definition SearchQueue_upds(f:TM->DecideResult)(q:SearchQueue)(n:N) :=
+get_SQ (N_iter_until (SearchQueue_upd f) (inl q) n).
+
+
+Definition SearchQueue_upd_bfs(f:TM->DecideResult)(q:SearchQueue):SearchQueue+SearchQueue :=
+let (q1,q2):=q in
+match q1 with
+| nil => inr q
+| x::q1' =>
+  inl
+  match f x.(tm) with
+  | Halt h => (q1',expand' x h ++ q2)
+  | NonHalt => (q1',q2)
+  | Unknown => (q1',x::q2)
+  end
+end.
+
+Definition SearchQueue_rst(q:SearchQueue):SearchQueue :=
+let (q1,q2):=q in (q1++q2,[]).
+
+Definition SearchQueue_upds_bfs(f:TM->DecideResult)(q:SearchQueue) :=
+SearchQueue_rst (get_SQ (N_iter_until (SearchQueue_upd_bfs f) (inl q) (length_tail (fst q)))).
+
+
+
+
+
+
+
+Definition decider(tm0:TM):DecideResult.
+Proof.
+  refine (
+    match TC_state.decide tm0 [([50]%N,20%nat);([50;100;200]%N,40%nat)] with
+    | (Halt h,_) => Halt h
+    | (NonHalt,_) => NonHalt
+    | (Unknown,_) => _
+    end).
+  refine (if (decide_nonhalt tm0 (NG 0 1 100 1 0 0 0 false)) then NonHalt else _).
+  refine (if (decide_nonhalt tm0 (NG 0 2 200 2 0 0 0 false)) then NonHalt else _).
+  refine (if (decide_nonhalt tm0 (NG 0 8 800 3 0 0 0 false)) then NonHalt else _).
+  refine (
+    match TC_state.decide tm0 [([2000]%N,O)] with
+    | (Halt h,_) => Halt h
+    | (NonHalt,_) => NonHalt
+    | (Unknown,_) => _
+    end).
+  refine (if (decide_nonhalt tm0 (NG 0 30 3000 3 2 4 0 true)) then NonHalt else _).
+  refine (if (decide_nonhalt tm0 (RWL_mod 0 30 3000 2 320 2 1 4 0)) then NonHalt else _).
+  refine (if (decide_nonhalt tm0 (RWL_mod 0 30 3000 3 320 2 1 4 0)) then NonHalt else _).
+  refine (if (decide_nonhalt tm0 (RWL_mod 0 30 3000 4 320 2 1 4 0)) then NonHalt else _).
+  refine (if (decide_nonhalt tm0 (RWL_mod 0 30 3000 6 320 2 1 4 0)) then NonHalt else _).
+  refine (
+    match TC_state.decide tm0 [([100000]%N,O)] with
+    | (Halt h,_) => Halt h
+    | (NonHalt,_) => NonHalt
+    | (Unknown,_) => _
+    end).
+  refine (if (decide_nonhalt tm0 (NG 0 30 3000 3 2 12 0 true)) then NonHalt else _).
+  refine (if (decide_nonhalt tm0 (CPS_LRU 0 30 3000 2 320 0 1 0 0)) then NonHalt else _).
+  refine (if (decide_nonhalt tm0 (CPS_LRU 0 30 3000 3 320 0 1 0 0)) then NonHalt else _).
+  refine (if (decide_nonhalt tm0 (CPS_LRU 0 30 3000 4 320 0 1 0 0)) then NonHalt else _).
+  refine (if (decide_nonhalt tm0 (CPS_LRU 0 30 3000 5 320 0 1 0 0)) then NonHalt else _).
+  refine (if (decide_nonhalt tm0 (CPS_LRU 0 30 3000 6 320 0 1 0 0)) then NonHalt else _).
+  refine (if (decide_nonhalt tm0 (CPS_LRU 0 30 3000 7 320 0 1 0 0)) then NonHalt else _).
+  refine (if (decide_nonhalt tm0 (CPS_LRU 0 30 3000 8 320 0 1 0 0)) then NonHalt else _).
+  refine (if (decide_nonhalt tm0 (CPS_LRU 0 30 3000 9 320 0 1 0 0)) then NonHalt else _).
+  refine (if (decide_nonhalt tm0 (CPS_LRU 0 30 3000 10 320 0 1 0 0)) then NonHalt else _).
+  refine (if (decide_nonhalt tm0 (CPS_LRU 0 30 3000 11 320 0 1 0 0)) then NonHalt else _).
+  refine (if (decide_nonhalt tm0 (CPS_LRU 0 30 3000 12 320 0 1 0 0)) then NonHalt else _).
+  refine (if (decide_nonhalt tm0 (NG 0 100 10000 2 4 0 0 true)) then NonHalt else _).
+  refine (if (decide_nonhalt tm0 (CPS_LRU 1001 100 10000 2 320 1 14 1 0)) then NonHalt else _).
+  refine (if (decide_nonhalt tm0 (RWL_mod 1001 30 3000 2 320 2 3 12 0)) then NonHalt else _).
+  refine (if (decide_nonhalt tm0 (NG 0 100 10000 3 8 8 0 true)) then NonHalt else _).
+  refine (if (decide_nonhalt tm0 (NG 0 100 10000 2 6 0 0 true)) then NonHalt else _).
+  refine (if (decide_nonhalt tm0 (RWL_mod 1001 10 1000 2 320 2 2 6 0)) then NonHalt else _).
+  refine (if (decide_nonhalt tm0 (RWL_mod 1001 1000 100000 1 320 2 2 4 0)) then NonHalt else _).
+  refine (if (decide_nonhalt tm0 (CPS_LRU 0 10 1000 4 320 0 3 1 0)) then NonHalt else _).
+  refine (if (decide_nonhalt tm0 (RWL_mod 1001 100 10000 6 320 2 2 8 0)) then NonHalt else _).
+  refine (
+    match TC_state.decide tm0 [([1000000]%N,O)] with
+    | (Halt h,_) => Halt h
+    | (NonHalt,_) => NonHalt
+    | (Unknown,_) => _
+    end).
+  refine Unknown.
+Defined.
+
+End TNF_Node.
+
+Import TNF_Node.
+
+Definition MAXT:=(2^60)%N.
+
+Definition q_0 := (N.iter 4 (SearchQueue_upds_bfs decider) root_1RB).
+Definition q_i l sz := (firstn sz (skipn l (fst q_0)),snd q_0).
+
+(*
+Compute (length_tail (fst q_0)).
+Time Definition q_1 := Eval native_compute in (SearchQueue_upds decider (q_i 0 100) MAXT).
+ *)
+
+Definition show_holdout (q:SearchQueue) := (List.map (fun x => TM_to_str x.(tm)) (snd q)).
+Definition holdout_i l sz := show_holdout (SearchQueue_upds decider (q_i l sz) MAXT).
+
+
