verify/HashTable.v
@@ -1,0 +1,700 @@
+Require Import Uint63.
+Require Import PArray.
+Require Import List.
+Require Import Lia.
+Require Import ZArith.
+From BusyCoq Require Import LibTactics.
+From BusyCoq Require Export Eqb.
+
+Module HashConcat.
+Open Scope uint63.
+Definition hash_t:Type := int*int.
+
+Definition hash_P:int := 1234577.
+Definition hash_v1:int := 293999.
+
+Definition hash_concat(a b:hash_t):hash_t :=
+let '(a0,a1):=a in
+let '(b0,b1):=b in
+(a0*b1+b0,a1*b1).
+
+Definition hv1:hash_t := Eval compute in (hash_v1*1,hash_P).
+Definition hv2:hash_t := Eval compute in (hash_v1*2,hash_P).
+Definition hv3:hash_t := Eval compute in (hash_v1*3,hash_P).
+Definition hv4:hash_t := Eval compute in (hash_v1*4,hash_P).
+Definition hv5:hash_t := Eval compute in (hash_v1*5,hash_P).
+Definition hv6:hash_t := Eval compute in (hash_v1*6,hash_P).
+Definition hv7:hash_t := Eval compute in (hash_v1*7,hash_P).
+Definition hv8:hash_t := Eval compute in (hash_v1*8,hash_P).
+Definition hv9:hash_t := Eval compute in (hash_v1*9,hash_P).
+Definition hv10:hash_t := Eval compute in (hash_v1*10,hash_P).
+Definition hv11:hash_t := Eval compute in (hash_v1*11,hash_P).
+Definition hv12:hash_t := Eval compute in (hash_v1*12,hash_P).
+Definition hv13:hash_t := Eval compute in (hash_v1*13,hash_P).
+Definition hv14:hash_t := Eval compute in (hash_v1*14,hash_P).
+Definition hv15:hash_t := Eval compute in (hash_v1*15,hash_P).
+Definition hv16:hash_t := Eval compute in (hash_v1*16,hash_P).
+
+Notation "a ## b" := (hash_concat a b) (at level 50, left associativity).
+Notation "a # b" := (a*hash_P+b)%uint63 (at level 50, left associativity).
+
+Fixpoint Pos_hash'(x:positive) h :=
+match x with
+| xH => h
+| xI x0 => Pos_hash' x0 (hv2 ## h)
+| xO x0 => Pos_hash' x0 (hv3 ## h)
+end.
+
+Definition Pos_hash(x:positive) := Pos_hash' x hv1.
+
+Definition N_hash(x:N) :=
+match x with
+| N0 => hv1
+| Npos x0 => hv2 ## Pos_hash x0
+end.
+
+Definition Z_hash(x:Z) :=
+match x with
+| Z0 => hv1
+| Zpos x0 => hv2 ## Pos_hash x0
+| Zneg x0 => hv3 ## Pos_hash x0
+end.
+
+Fixpoint list_hash'{A}(f:A->_)(ls:list A) h:=
+match ls with
+| nil => h
+| a::ls0 => list_hash' f ls0 (hv1 ## f a ## h)
+end.
+
+Definition list_hash{A} f (ls:list A) := list_hash' f ls hv2.
+
+Definition prod_hash{A B} f g (x:A*B) :=
+  let (a,b):=x in hv1 ## (f a) ## (g b).
+
+Definition bool_hash(x:bool) :=
+match x with
+| true => hv1
+| false => hv2
+end.
+
+Class Hash A := {
+  hash : A -> (int*int)
+}.
+
+#[export] Instance bool_Hash: Hash bool := (ltac: (split; apply bool_hash)).
+#[export] Instance positive_Hash: Hash positive := (ltac: (split; apply Pos_hash)).
+#[export] Instance N_Hash: Hash N := (ltac: (split; apply N_hash)).
+#[export] Instance Z_Hash: Hash Z := (ltac: (split; apply Z_hash)).
+#[export] Instance list_Hash A: Hash A -> Hash (list A) := (ltac: (esplit; apply list_hash,hash)).
+#[export] Instance prod_Hash A B: Hash A -> Hash B -> Hash (A*B) := (ltac: (esplit; apply prod_hash; apply hash)).
+
+End HashConcat.
+
+
+
+Module Type HashableType.
+Parameter K:Type.
+Parameter K_hash:K->(int*int).
+Parameter K_eq:K->K->bool.
+Parameter K_eq_spec:forall a b, Bool.reflect (a=b) (K_eq a b).
+End HashableType.
+
+Module ListHash(A:HashableType) <: HashableType.
+Import HashConcat.
+Definition K:Type := list A.K.
+Definition K_hash(x:K):int*int := list_hash A.K_hash x.
+Definition K_eq := list_eqb A.K_eq.
+Definition K_eq_spec a b := list_eqb_spec A.K_eq a b A.K_eq_spec.
+End ListHash.
+
+Module ProdHash(A:HashableType)(B:HashableType) <: HashableType.
+Import HashConcat.
+Definition K:Type := A.K*B.K.
+Definition K_hash(x:K):int*int :=
+  let '(a,b):=x in
+  A.K_hash a ## B.K_hash b.
+Definition K_eq := prod_eqb A.K_eq B.K_eq.
+Definition K_eq_spec a b := prod_eqb_spec A.K_eq B.K_eq a b A.K_eq_spec B.K_eq_spec.
+End ProdHash.
+
+Module Type ValueType.
+Parameter V:Type.
+End ValueType.
+
+Module HashMap(KeyType:HashableType)(ValueType:ValueType).
+Export KeyType.
+Export ValueType.
+Definition hmap_t := array (list (K*V*int)).
+
+Open Scope uint63.
+
+Definition hmap_make(len:int):hmap_t :=
+  make (if len=?0 then 1 else len) nil.
+
+Fixpoint hmap_entry_set(ls:list (K*V*int))(k:K)(v:V)(x:int) :=
+match ls with
+| nil => (k,v,x)::nil
+| ((k',v',x') as h)::t =>
+    if (if (x' =? x) then (K_eq k' k) else false) then (k,v,x)::t
+    else h::(hmap_entry_set t k v x)
+end.
+
+Fixpoint hmap_entry_get(ls:list (K*V*int))(k:K)(x:int) :=
+match ls with
+| nil => None
+| ((k',v',x') as h)::t =>
+    if (if (x' =? x) then (K_eq k' k) else false) then Some v'
+    else hmap_entry_get t k x
+end.
+
+Definition hmap_set(k:K)(v:V)(c:hmap_t):hmap_t :=
+let x:=fst (K_hash k) in
+let p:=(x mod (PArray.length c)) in
+c.[p<-hmap_entry_set c.[p] k v x].
+
+Definition hmap_get(k:K)(c:hmap_t):option V :=
+let x:=fst (K_hash k) in
+let p:=(x mod (PArray.length c)) in
+hmap_entry_get c.[p] k x.
+
+Definition hmap_set'(k:K)(v:V)(c:hmap_t) x p:hmap_t :=
+c.[p<-hmap_entry_set c.[p] k v x].
+
+Definition hmap_get'(k:K)(c:hmap_t) x p:option V :=
+hmap_entry_get c.[p] k x.
+
+Definition hmap_WF(c:hmap_t):Prop :=
+  (0 <? (PArray.length c)) = true.
+
+Lemma hmap_make_WF len:
+  hmap_WF (hmap_make len).
+Proof.
+  unfold hmap_WF.
+  cbn.
+  rewrite length_make.
+  destruct (len =? 0) eqn:E.
+  1: reflexivity.
+  destruct (len ≤? max_length).
+  2: reflexivity.
+  rewrite ltb_spec.
+  destruct (eqbP len 0) as [E0|E0].
+  1: congruence.
+  pose proof (to_Z_bounded len).
+  change (to_Z 0) with BinInt.Z0.
+  change (to_Z 0) with BinInt.Z0 in E0.
+  lia.
+Qed.
+
+Lemma hmap_set_WF k v c:
+  hmap_WF c ->
+  hmap_WF (hmap_set k v c).
+Proof.
+  unfold hmap_WF.
+  intros H.
+  unfold hmap_set.
+  rewrite length_set.
+  apply H.
+Qed.
+
+Lemma hmap_get_set_same k v c:
+  hmap_WF c ->
+  hmap_get k (hmap_set k v c) = Some v.
+Proof.
+  intros Hwf.
+  unfold hmap_WF in Hwf.
+  rewrite ltb_spec in Hwf.
+  unfold hmap_get,hmap_set.
+  rewrite length_set.
+  remember (fst (K_hash k) mod PArray.length c) as x.
+  rewrite get_set_same.
+  2:{
+    rewrite Heqx.
+    rewrite ltb_spec.
+    rewrite mod_spec.
+    apply BinInt.Z.mod_pos_bound.
+    apply Hwf.
+  }
+  induction c.[x] as [|[[k0 v0] x0] t].
+  - cbn.
+    rewrite eqb_refl.
+    destruct (K_eq_spec k k); trivial; congruence.
+  - cbn.
+    destruct (x0 =? fst (K_hash k)) eqn:Ex0k.
+    + destruct (K_eq_spec k0 k) as [Ek0|Ek0].
+      * cbn.
+        rewrite eqb_refl.
+        destruct (K_eq_spec k k); congruence.
+      * cbn.
+        rewrite Ex0k.
+        destruct (K_eq_spec k0 k); congruence.
+    + cbn.
+      rewrite Ex0k.
+      apply IHt.
+Qed.
+
+Lemma hmap_get_set_other k k' v c:
+  hmap_WF c ->
+  k<>k' ->
+  hmap_get k (hmap_set k' v c) = hmap_get k c.
+Proof.
+  intros Hwf.
+  unfold hmap_WF in Hwf.
+  rewrite ltb_spec in Hwf.
+  unfold hmap_get,hmap_set.
+  rewrite length_set.
+  remember (fst (K_hash k') mod PArray.length c) as x'.
+  remember (fst (K_hash k) mod PArray.length c) as x.
+  intros Hne.
+  destruct (eq_dec x x').
+  2: rewrite get_set_other; auto.
+  clear Heqx'. subst x'.
+  rewrite get_set_same.
+  2:{
+    rewrite Heqx.
+    rewrite ltb_spec.
+    rewrite mod_spec.
+    apply BinInt.Z.mod_pos_bound.
+    apply Hwf.
+  }
+  induction c.[x] as [|[[k0 v0] x0] t].
+  - cbn.
+    destruct (fst (K_hash k') =? fst (K_hash k)); trivial.
+    destruct (K_eq_spec k' k); trivial.
+    congruence.
+  - cbn.
+    cbn in IHt.
+    destruct (x0 =? fst (K_hash k')) eqn:Ex0k'.
+    + destruct (K_eq_spec k0 k') as [Ek0|Ek0].
+      * destruct (x0 =? fst (K_hash k)) eqn:Ex0k.
+        -- cbn.
+          rewrite Uint63.eqb_spec in Ex0k,Ex0k'.
+          rewrite <-Ex0k,Ex0k'.
+          rewrite eqb_refl,Ek0.
+          destruct (K_eq_spec k' k); congruence.
+        -- cbn.
+          destruct (fst (K_hash k') =? fst (K_hash k)) eqn:Ek'k.
+          2: reflexivity.
+          rewrite Uint63.eqb_spec in Ex0k',Ek'k.
+          rewrite eqb_false_spec in Ex0k.
+          congruence.
+      * cbn.
+        destruct (x0 =? fst (K_hash k)) eqn:Ex0k; auto.
+        destruct (K_eq_spec k0 k) as [Ek1|Ek1]; auto.
+    + cbn.
+      destruct (x0 =? fst (K_hash k)) eqn:Ex0k; auto.
+      destruct (K_eq_spec k0 k) as [Ek1|Ek1]; auto.
+Qed.
+
+Lemma hmap_get_make k len:
+  hmap_get k (hmap_make len) = None.
+Proof.
+  cbn.
+  rewrite get_make.
+  reflexivity.
+Qed.
+
+Definition hmap_upd2{T}(k:K)(f:option V->V*T)(c:hmap_t):hmap_t*T :=
+let x:=fst (K_hash k) in
+let p:=(x mod (PArray.length c)) in
+let (v,t):=(f (hmap_get' k c x p)) in
+(hmap_set' k v c x p,t).
+
+Lemma hmap_upd2_spec{T} k (f:option V->V*T) c:
+  hmap_upd2 k f c =
+  let (v,t):=(f (hmap_get k c)) in
+  (hmap_set k v c,t).
+Proof.
+  reflexivity.
+Qed.
+
+Definition hmap_upd(k:K)(f:option V->V)(c:hmap_t):hmap_t :=
+let x:=fst (K_hash k) in
+let p:=(x mod (PArray.length c)) in
+(hmap_set' k (f (hmap_get' k c x p)) c x p).
+
+Lemma hmap_upd_spec k f c:
+  hmap_upd k f c =
+  (hmap_set k (f (hmap_get k c)) c).
+Proof.
+  reflexivity.
+Qed.
+
+Definition hmap_add(k:K)(v:V)(c:hmap_t):option hmap_t :=
+let x:=fst (K_hash k) in
+let p:=(x mod (PArray.length c)) in
+match hmap_get' k c x p with
+| None =>
+  Some (hmap_set' k v c x p)
+| Some _ => None
+end.
+
+Lemma hmap_add_spec k v c:
+hmap_add k v c =
+match hmap_get k c with
+| None => Some (hmap_set k v c)
+| Some _ => None
+end.
+Proof.
+  reflexivity.
+Qed.
+
+
+Section Cached.
+Hypothesis f:K->V.
+Definition hmap_get_cached'(k:K)(c:hmap_t):V*hmap_t :=
+match hmap_get k c with
+| Some v => (v,c)
+| None =>
+  let v := f k in
+  (v,hmap_set k v c)
+end.
+
+Definition hmap_get_cached(k:K)(c:hmap_t):V*hmap_t :=
+let x:=fst (K_hash k) in
+let p:=(x mod (PArray.length c)) in
+match hmap_get' k c x p with
+| Some v => (v,c)
+| None =>
+  let v := f k in
+  (v,hmap_set' k v c x p)
+end.
+
+Definition cache_WF(c:hmap_t):Prop :=
+hmap_WF c /\
+forall k,
+match hmap_get k c with
+| None => True
+| Some v => v = f k
+end.
+
+
+Lemma hmap_get_cached'_spec k c:
+  hmap_get_cached k c =
+  hmap_get_cached' k c.
+Proof.
+  reflexivity.
+Qed.
+
+Lemma hmap_get_cached_spec k c:
+  cache_WF c ->
+  let '(v,c') := hmap_get_cached k c in
+  v = f k /\
+  cache_WF c'.
+Proof.
+  unfold cache_WF.
+  intros [Hwf1 Hwf2].
+  rewrite hmap_get_cached'_spec.
+  unfold hmap_get_cached'.
+  destruct (hmap_get k c) eqn:E.
+  - pose proof (Hwf2 k) as Hwf.
+    rewrite E in Hwf.
+    tauto.
+  - split.
+    1: reflexivity.
+    split.
+    1: apply hmap_set_WF,Hwf1.
+    intros k0.
+    destruct (K_eq_spec k0 k).
+    1: subst k0; rewrite hmap_get_set_same; auto.
+    rewrite hmap_get_set_other; auto.
+    apply Hwf2.
+Qed.
+
+Lemma hmap_make_cache_WF len:
+  cache_WF (hmap_make len).
+Proof.
+  split.
+  1: apply hmap_make_WF.
+  intros k.
+  rewrite hmap_get_make; trivial.
+Qed.
+End Cached.
+End HashMap.
+
+
+Module Uint63_K <: HashableType.
+Definition K := int.
+Definition K_hash(x:int) := (x,HashConcat.hash_P).
+Definition K_eq := Uint63.eqb.
+Lemma K_eq_spec x y: Bool.reflect (x=y) (Uint63.eqb x y).
+Proof.
+  destruct (Uint63.eqb x y) eqn:E.
+  - rewrite Uint63.eqb_spec in E.
+    constructor.
+    apply E.
+  - rewrite eqb_false_spec in E.
+    constructor.
+    apply E.
+Qed.
+End Uint63_K.
+
+Module Uint63_V <: ValueType.
+Definition V := int.
+End Uint63_V.
+
+Module IdAlloc(K_t:HashableType).
+Export K_t.
+
+Module V_t <: ValueType.
+Definition V := K.
+End V_t.
+
+Module MapToId := HashMap K_t Uint63_V.
+Module MapFromId := HashMap Uint63_K V_t.
+Import ZArith.
+
+Definition id_alloc_t:Type := MapToId.hmap_t*MapFromId.hmap_t*int.
+Definition max_id:int := 1000000000000000000.
+
+Definition id_alloc_make(len:int):id_alloc_t := (MapToId.hmap_make len,MapFromId.hmap_make len,0%uint63).
+
+Definition get_key(x:int)(c:id_alloc_t):option K :=
+let '(mp1,mp2,p) := c in
+MapFromId.hmap_get x mp2.
+
+Definition get_id(x:K)(c:id_alloc_t):option int :=
+let '(mp1,mp2,p) := c in
+MapToId.hmap_get x mp1.
+
+Definition get_or_alloc_id(x:K)(c:id_alloc_t):option (int*id_alloc_t) :=
+let '(mp1,mp2,p) := c in
+match MapToId.hmap_get x mp1 with
+| Some y => Some (y,c)
+| None =>
+  if (p <? max_id)%uint63 then
+    Some (p,(MapToId.hmap_set x p mp1,MapFromId.hmap_set p x mp2,(p+1)%uint63))
+  else None
+end.
+
+Definition id_alloc_WF(c:id_alloc_t):Prop :=
+let '(mp1,mp2,p) := c in
+MapToId.hmap_WF mp1 /\
+MapFromId.hmap_WF mp2 /\
+(forall x y, get_id x c = Some y <-> get_key y c = Some x) /\
+(forall x,
+match get_id x c with
+| None => True
+| Some y => (y <? p)%uint63 = true
+end) /\
+(0 <= φ (p)%uint63 + 1 < wB)%Z.
+
+Lemma id_alloc_make_WF len:
+id_alloc_WF (id_alloc_make len).
+Proof.
+  unfold id_alloc_WF,id_alloc_make.
+  split.
+  1: apply MapToId.hmap_make_WF.
+  split.
+  1: apply MapFromId.hmap_make_WF.
+  unfold get_id,get_key.
+  split;[|split].
+  - intros x y.
+    rewrite MapToId.hmap_get_make.
+    rewrite MapFromId.hmap_get_make.
+    split; congruence.
+  - intros x.
+    rewrite MapToId.hmap_get_make; trivial.
+  - cbv. split; congruence.
+Qed.
+
+Lemma get_or_alloc_id_WF x c:
+id_alloc_WF c ->
+match get_or_alloc_id x c with
+| None => True
+| Some (y,c') =>
+  get_id x c' = Some y /\
+  id_alloc_WF c' /\
+  (forall x', x'<>x -> get_id x' c' = get_id x' c)
+end.
+Proof.
+  unfold id_alloc_WF,get_or_alloc_id.
+  destruct c as [[mp1 mp2] p].
+  intros [Hwf1 [Hwf2 [Hwf3 [Hwf4 Hwf5]]]].
+  destruct (MapToId.hmap_get x mp1) eqn:E1.
+  - split.
+    1: apply E1.
+    split.
+    1: tauto.
+    intros.
+    reflexivity.
+  - destruct (p <? max_id)%uint63 eqn:Ep; trivial.
+    split.
+    1: apply MapToId.hmap_get_set_same,Hwf1.
+    split.
+    + split.
+      1: apply MapToId.hmap_set_WF,Hwf1.
+      split.
+      1: apply MapFromId.hmap_set_WF,Hwf2.
+      split;[|split]. 2: {
+        intros x'.
+        unfold get_id.
+        destruct (K_eq_spec x' x).
+        - subst x'.
+          rewrite MapToId.hmap_get_set_same; auto.
+          rewrite ltb_spec,add_spec.
+          rewrite to_Z_1.
+          rewrite Z.mod_small.
+          1: lia.
+          apply Hwf5.
+        - rewrite MapToId.hmap_get_set_other; auto.
+          specialize (Hwf4 x').
+          unfold get_id in Hwf4.
+          destruct (MapToId.hmap_get x' mp1); trivial.
+          generalize Hwf4.
+          do 2 rewrite ltb_spec.
+          rewrite add_spec,Z.mod_small; auto.
+          rewrite to_Z_1.
+          lia.
+      }
+      2: {
+        rewrite add_spec,to_Z_1,Z.mod_small; auto.
+        rewrite ltb_spec in Ep.
+        eassert (φ (max_id) = _)%uint63 as E by (cbv; reflexivity).
+        rewrite E in Ep; clear E.
+        eassert (wB = _)%uint63 as E by (cbv; reflexivity).
+        rewrite E; clear E.
+        lia.
+      }
+      intros x' y.
+      specialize (Hwf3 x' y).
+      destruct (K_eq_spec x' x).
+      * subst x'.
+        unfold get_id,get_key.
+        rewrite MapToId.hmap_get_set_same; auto.
+        destruct (Uint63_K.K_eq_spec p y).
+        -- subst y.
+          rewrite MapFromId.hmap_get_set_same; auto.
+          tauto.
+        -- split.
+          1: congruence.
+          intro H.
+          rewrite MapFromId.hmap_get_set_other in H; auto.
+          unfold get_id,get_key in Hwf3.
+          rewrite <-Hwf3 in H.
+          congruence.
+      * unfold get_id,get_key.
+        unfold get_id,get_key in Hwf3.
+        rewrite MapToId.hmap_get_set_other; auto.
+        rewrite Hwf3.
+        destruct (Uint63_K.K_eq_spec p y).
+        -- subst y.
+          rewrite MapFromId.hmap_get_set_same; auto.
+          rewrite <-Hwf3.
+          specialize (Hwf4 x').
+          unfold get_id in Hwf4.
+          split. 2: congruence.
+          intros H.
+          rewrite H,ltb_spec in Hwf4.
+          lia.
+        -- rewrite MapFromId.hmap_get_set_other; auto.
+          tauto.
+    + intros x' Hne.
+      unfold get_id.
+      apply MapToId.hmap_get_set_other; tauto.
+Qed.
+
+End IdAlloc.
+
+
+Module HashMultimap(K_t:HashableType)(V_t:ValueType).
+
+Module list_V_t <: ValueType.
+Definition V := list V_t.V.
+End list_V_t.
+
+Module list_V_HashMap := HashMap K_t list_V_t.
+Export K_t.
+Export V_t.
+
+Definition hmap_t := list_V_HashMap.hmap_t.
+
+Definition hmap_make(len:int):hmap_t :=
+list_V_HashMap.hmap_make len.
+
+Definition hmap_get(x:K)(c:hmap_t):list V :=
+match list_V_HashMap.hmap_get x c with
+| Some ls => ls
+| None => nil
+end.
+
+Definition hmap_add(x:K)(y:V)(c:hmap_t):hmap_t :=
+list_V_HashMap.hmap_upd x (fun ls =>
+y::match ls with
+| None => nil
+| Some ls0 => ls0
+end) c.
+
+Definition hmap_WF(c:hmap_t):Prop :=
+list_V_HashMap.hmap_WF c.
+
+Lemma hmap_make_WF len:
+  hmap_WF (hmap_make len).
+Proof.
+  apply list_V_HashMap.hmap_make_WF.
+Qed.
+
+Lemma hmap_get_make x' len:
+hmap_get x' (hmap_make len) = nil.
+Proof.
+  unfold hmap_get,hmap_make.
+  rewrite list_V_HashMap.hmap_get_make.
+  reflexivity.
+Qed.
+
+Lemma hmap_add_WF x y c:
+hmap_WF c ->
+hmap_WF (hmap_add x y c).
+Proof.
+  unfold hmap_WF,hmap_add.
+  rewrite list_V_HashMap.hmap_upd_spec.
+  apply list_V_HashMap.hmap_set_WF.
+Qed.
+
+Lemma hmap_get_add_same x y c:
+hmap_WF c ->
+hmap_get x (hmap_add x y c) = y::(hmap_get x c).
+Proof.
+  unfold hmap_WF,hmap_get,hmap_add.
+  intro Hwf.
+  rewrite list_V_HashMap.hmap_upd_spec.
+  rewrite list_V_HashMap.hmap_get_set_same; auto.
+Qed.
+
+Lemma hmap_get_add_other x y c x':
+hmap_WF c ->
+x'<> x ->
+hmap_get x' (hmap_add x y c) = (hmap_get x' c).
+Proof.
+  unfold hmap_WF,hmap_get,hmap_add.
+  intros Hwf Hne.
+  rewrite list_V_HashMap.hmap_upd_spec.
+  rewrite list_V_HashMap.hmap_get_set_other; auto.
+Qed.
+
+Lemma hmap_get_add_mono x y c x' x'':
+hmap_WF c ->
+In x'' (hmap_get x' c) ->
+In x'' (hmap_get x' (hmap_add x y c)).
+Proof.
+  intros Hwf Hin.
+  destruct (K_eq_spec x' x).
+  - subst.
+    rewrite hmap_get_add_same; auto.
+    right; auto.
+  - rewrite hmap_get_add_other; auto.
+Qed.
+
+End HashMultimap.
+
+
+
+
+
+
+
+
+
+
+
+
+
