verify/TC.v
@@ -1,0 +1,779 @@
+Require Import ZArith.
+Require Import List.
+Require Import Lia.
+Require Uint63.
+From BusyCoq Require Import HashTable.
+From BusyCoq Require TM.
+From BusyCoq Require Import Eqb.
+From Coq Require Import Lists.Streams.
+From Coq Require Import Lists.List.
+
+Ltac destruct_spec_expr e f :=
+match e with
+| match ?a with _ => _ end => destruct_spec_expr a f
+| if ?a then _ else _ => destruct_spec_expr a f
+| ?a ?arg1 ?arg2 ?arg3 ?arg4 ?arg5 ?arg6 ?arg7 =>
+  pose proof (f arg1 arg2 arg3 arg4 arg5 arg6 arg7);
+  destruct e
+| ?a ?arg1 ?arg2 ?arg3 ?arg4 ?arg5 ?arg6 =>
+  pose proof (f arg1 arg2 arg3 arg4 arg5 arg6);
+  destruct e
+| ?a ?arg1 ?arg2 ?arg3 ?arg4 ?arg5 =>
+  pose proof (f arg1 arg2 arg3 arg4 arg5);
+  destruct e
+| ?a ?arg1 ?arg2 ?arg3 ?arg4 =>
+  pose proof (f arg1 arg2 arg3 arg4);
+  destruct e
+| ?a ?arg1 ?arg2 ?arg3 =>
+  pose proof (f arg1 arg2 arg3);
+  destruct e
+| ?a ?arg1 ?arg2 =>
+  pose proof (f arg1 arg2);
+  destruct e
+| ?a ?arg1 =>
+  pose proof (f arg1);
+  destruct e
+end.
+
+Ltac destruct_spec f :=
+match goal with
+|- ?a => destruct_spec_expr a f
+end.
+Module Uint.
+Import Uint63.
+Open Scope uint63.
+Definition uint_0 := 0x0.
+Definition uint_1 := 0x1.
+
+#[export]
+Instance uint_Eqb: Eqb int.
+Proof.
+  apply Build_Eqb with (eqb:=eqb).
+  intros.
+  pose proof (eqb_spec x y) as H.
+  destruct (x=?y); constructor.
+  1: tauto.
+  intro.
+  rewrite <-H in H0.
+  congruence.
+Defined.
+
+Fixpoint to_Pos_rec(x:int)(n:nat) :=
+if x =? 0x1 then xH else
+match n with
+| O => xH
+| S n0 =>
+  let y := (to_Pos_rec (x>>0x1) n0) in
+  (if is_even x then y~0 else y~1)%positive
+end.
+
+Definition to_N(x:int) :=
+if x=?0x0 then N0 else Npos (to_Pos_rec x size).
+
+End Uint.
+
+Import TM.
+Module TC(Ctx:Ctx).
+Module TM := TM Ctx.
+Export TM.
+
+Import Uint.
+
+Module BoundedConfig.
+Record T := {
+  l: list Sym;
+  r: list Sym;
+  s: Q;
+  sgn: dir;
+}.
+
+Definition T_eqb(a b:T) :=
+let (l1,r1,s1,sgn1):=a in
+let (l2,r2,s2,sgn2):=b in
+((eqb s1 s2) && (eqb sgn1 sgn2) && (eqb l1 l2) && (eqb r1 r2))%bool.
+
+#[export]
+Instance T_Eqb: Eqb T.
+Proof.
+  apply Build_Eqb with (eqb:=T_eqb).
+  intros.
+  destruct x,y.
+  unfold T_eqb.
+  destruct (eqb_spec s2 s3); solve_Bool_reflect.
+  destruct (eqb_spec sgn0 sgn1); solve_Bool_reflect.
+  destruct (eqb_spec l0 l1); solve_Bool_reflect.
+  destruct (eqb_spec r0 r1); solve_Bool_reflect.
+Defined.
+
+
+Definition T0:T := Build_T [] [] q0 R.
+
+Definition to_config (x:T) (l0 r0:side) :=
+let (l,r,s,sgn):=x in
+match sgn with
+| L => l0 <* r <{{s}} l *> r0
+| R => l0 <* l {{s}}> r *> r0
+end.
+
+Definition to_config' (x:T) :=
+let (l,r,s,sgn):=x in
+match sgn with
+| L => const s0 <* r <{{s}} l *> const s0
+| R => const s0 <* l {{s}}> r *> const s0
+end.
+
+Definition step(tm:TM)(x:T):option (T*(Q*Sym)) :=
+let (l,r,s,sgn):=x in
+match r with
+| nil => None
+| m::r0 =>
+  match tm (s,m) with
+  | None => None
+  | Some (m',sgn',s') =>
+    if dir_eqb sgn sgn' then
+      Some (Build_T (m'::l) r0 s' sgn',(s,m))
+    else
+      Some (Build_T (m'::r0) l s' sgn',(s,m))
+  end
+end.
+
+Definition step1(tm:TM)(x:T):T+T :=
+match step tm x with
+| Some (x',_) => inl x'
+| None => inr x
+end.
+
+Definition multistep(tm:TM)(x:T)(n:N):T+T :=
+N_iter_until (step1 tm) (inl x) n.
+
+Definition progress(tm:TM)(x:T)(n:N):T+T :=
+match n with
+| N0 => inr x
+| _ => multistep tm x n
+end.
+
+Definition ht_r(ls:list Sym):Sym*(list Sym) :=
+match ls with
+| nil => (s0,nil)
+| h::t => (h,t)
+end.
+
+Definition T':Type := T*(nat*nat*nat*nat).
+
+Definition step'(tm:TM)(x:T'):T' :=
+let '(x0,(ld1,rd1,ld2,rd2)):=x in
+let (l,r,s,sgn):=x0 in
+let (m,r0):=ht_r r in
+match tm (s,m) with
+| None => x
+| Some (m',sgn',s') =>
+  if dir_eqb sgn sgn' then
+    (Build_T (m'::l) r0 s' sgn',
+    match rd2 with
+    | O => (ld1,S rd1,S ld2,O)
+    | S rd2' => (ld1,rd1,S ld2,rd2')
+    end)
+  else
+    (Build_T (m'::r0) l s' sgn',
+    match rd2 with
+    | O => (S rd1,ld1,S O,ld2)
+    | S rd2' => (rd1,ld1,rd2,ld2)
+    end)
+end.
+
+Definition steps'(tm:TM)(x:T)(n:N):T':=
+N.iter n (step' tm) (x,(O,O,O,O)).
+
+Definition step_d(tm:TM)(x:T*Uint63.int):option (T*Uint63.int) :=
+let (x1,x2):=x in
+let (l,r,s,sgn):=x1 in
+match r with
+| nil => None
+| m::r0 =>
+  match tm (s,m) with
+  | None => None
+  | Some (m',sgn',s') =>
+    let x2':=
+      match sgn' with
+      | R => Uint63.add x2 uint_1
+      | L => Uint63.sub x2 uint_1
+      end in
+    if dir_eqb sgn sgn' then
+      Some (Build_T (m'::l) r0 s' sgn',x2')
+    else
+      Some (Build_T (m'::r0) l s' sgn',x2')
+  end
+end.
+
+Fixpoint find_cycle_0(tm:TM)(x0:T)(x1:T*Uint63.int)(n:nat) :=
+match n with
+| O => false
+| S n0 =>
+  match step_d tm x1 with
+  | None => false
+  | Some (x2a,x2b) =>
+    if ((eqb x2b uint_0) && (eqb x0 x2a))%bool then
+      true
+    else
+      find_cycle_0 tm x0 (x2a,x2b) n0
+  end
+end.
+
+Definition find_cycle(tm:TM)(x:T)(n:nat) :=
+  find_cycle_0 tm x (x,uint_0) n.
+
+End BoundedConfig.
+
+
+Module TC_state.
+Import HashConcat.
+Record T := {
+  bc: BoundedConfig.T;
+  t0: Uint63.int;
+  h0: hash_t;
+  hs: list (Uint63.int*dir*(hash_t))
+}.
+Definition upd(tm:TM)(x:T):T+(T*(Q*Sym)) :=
+let (bc,t0,h0,hs):=x in
+match BoundedConfig.step tm bc with
+| Some (bc',h) => inl (Build_T bc' (Uint63.succ t0) ((hash h) ## h0) hs)
+| None =>
+  let (l,r,s,sgn):=bc in
+  match r with
+  | nil => inl (Build_T (BoundedConfig.Build_T l [s0] s sgn) uint_0 hv1 ((t0,sgn,h0)::hs))
+  | m0::r0 => inr (x,(s,m0))
+  end
+end.
+
+Definition upds(tm:TM)(x:T)(n:N) :=
+  N_iter_until (upd tm) (inl x) n.
+
+Definition T0:T := Build_T BoundedConfig.T0 uint_0 hv1 [].
+
+Fixpoint check_TC_0(ls1 ls2:list (Uint63.int*dir*(hash_t)))(n:nat):bool :=
+match n with
+| O => true
+| S n0 =>
+  match ls1,ls2 with
+  | h1::t1,h2::t2 => (eqb h1 h2) && check_TC_0 t1 t2 n0
+  | _,_ => false
+  end
+end.
+
+Fixpoint get_TC_period(ls:list (Uint63.int*dir*(hash_t)))(n:nat):Uint63.int :=
+match n with
+| O => uint_0
+| S n0 =>
+  match ls with
+  | nil => uint_0
+  | (h0,h1,h2)::t => Uint63.add h0 (get_TC_period t n0)
+  end
+end.
+
+Fixpoint check_TC_1(ls1 ls2:list (Uint63.int*dir*(hash_t)))(n:nat):option (Uint63.int*nat) :=
+match ls2 with
+| nil => None
+| h2::t2 =>
+  if (check_TC_0 ls1 ls2 n) then Some (get_TC_period ls1 n,n) else (check_TC_1 ls1 t2 (S n))
+end.
+
+Definition check_TC_2(ls:list (Uint63.int*dir*(hash_t))):option (Uint63.int*nat) :=
+  check_TC_1 ls (List.tl ls) (S O).
+
+Definition check_TC(tm:TM)(x:T):bool :=
+match check_TC_2 x.(hs) with
+| Some (p,d) =>
+  let p' := (to_N p) in
+  let '(ld1,rd1,_,_) := snd (BoundedConfig.steps' tm x.(bc) p') in
+  let (l,r,s,sgn):=x.(bc) in
+  match x.(hs) with
+  | nil => false
+  | (_,sgn0,_)::_ =>
+    if eqb sgn sgn0 then
+      let l1:=firstn ld1 l in
+      let r1:=r++(repeat s0 d) in
+      let c1:=BoundedConfig.Build_T l1 r1 s sgn in
+      match BoundedConfig.progress tm c1 p' with
+      | inl (BoundedConfig.Build_T l2 r2 s2 sgn2) =>
+        ((eqb s2 s) && (eqb sgn2 sgn) && (eqb r2 r) && (eqb l2 (l1++(skipn (length l1) l2))))%bool
+      | _ => false
+      end
+    else
+      let r1:=firstn rd1 r in
+      let l1:=l++(repeat s0 d) in
+      let c1:=BoundedConfig.Build_T l1 r1 s sgn in
+      match BoundedConfig.progress tm c1 p' with
+      | inl (BoundedConfig.Build_T l2 r2 s2 sgn2) =>
+        ((eqb s2 s) && (eqb sgn2 sgn) && (eqb l2 l) && (eqb r2 (r1++(skipn (length r1) r2))))%bool
+      | _ => false
+      end
+  end
+| None => false
+end.
+
+Fixpoint decide_0(tm:TM)(ls:list N)(x:T):DecideResult*T :=
+match ls with
+| nil => (Unknown,x)
+| n::t =>
+  match upds tm x n with
+  | inr (x',h) => (Halt h,x')
+  | inl x' =>
+    if check_TC tm x' then (NonHalt,x') else decide_0 tm t x'
+  end
+end.
+
+Fixpoint decide_1(tm:TM)(ls:list ((list N)*nat))(x:T):DecideResult*T :=
+match ls with
+| nil => (Unknown,x)
+| (n,n0)::t =>
+  let res := decide_0 tm n x in
+  match res with
+  | (Unknown,x') =>
+    if BoundedConfig.find_cycle tm x'.(bc) n0 then (NonHalt,x')
+    else decide_1 tm t x'
+  | _ => res
+  end
+end.
+
+Definition decide(tm:TM)(ls:list ((list N)*nat)):DecideResult*T :=
+  decide_1 tm ls T0.
+
+End TC_state.
+
+
+Section tm_ctx.
+Hypothesis tm:TM.
+
+Lemma BoundedConfig_step_spec x:
+match BoundedConfig.step tm x with
+| None =>
+    x.(BoundedConfig.r) = nil \/
+    forall l r,
+    halted tm (BoundedConfig.to_config x l r)
+| Some (x',h) =>
+    forall l r,
+    (BoundedConfig.to_config x l r) -[ tm ]-> (BoundedConfig.to_config x' l r)
+end.
+Proof.
+  destruct x as [l [|m r] s sgn]; cbn; trivial.
+  - left; reflexivity.
+  - destruct (tm (s,m)) as [[[m' sgn'] s']|] eqn:E; trivial.
+    + destruct sgn,sgn'; cbn; intros; constructor; apply E.
+    + right. intros.
+      destruct sgn; apply E.
+Qed.
+
+Definition f_if_inl{S S'}(f:S->S+S') a :=
+match a with
+| inl a0 => f a0
+| inr a0 => a
+end.
+
+Lemma N_iter_until_spec' {S S'} (f:S->S+S') x n:
+  N_iter_until f x n =
+  N.iter n (f_if_inl f) x.
+Proof.
+  rewrite Nnat.N2Nat.inj_iter.
+  destruct n.
+  1: reflexivity.
+  cbn[N.to_nat].
+  cbn[N_iter_until].
+  gen x.
+  induction p; intros; cbn.
+  - destruct x.
+    + rewrite IHp.
+      rewrite IHp.
+      replace (Pos.to_nat (p~1)) with ((Pos.to_nat p)+(Pos.to_nat p)+1) by lia.
+      repeat rewrite Nat.iter_add.
+      reflexivity.
+    + generalize (Pos.to_nat p~1) as n.
+      induction n.
+      1: reflexivity.
+      rewrite Nat.iter_succ,<-IHn.
+      reflexivity.
+  - destruct x.
+    rewrite IHp.
+    rewrite IHp.
+    + replace (Pos.to_nat (p~0)) with ((Pos.to_nat p)+(Pos.to_nat p)) by lia.
+      repeat rewrite Nat.iter_add.
+      reflexivity.
+    + generalize (Pos.to_nat p~0) as n.
+      induction n.
+      1: reflexivity.
+      rewrite Nat.iter_succ,<-IHn.
+      reflexivity.
+  - replace (Pos.to_nat 1) with 1 by lia.
+    destruct x; reflexivity.
+Qed.
+
+
+Lemma BoundedConfig_multistep_spec x n:
+match BoundedConfig.multistep tm x n with
+| inl x' =>
+    forall l r,
+    (BoundedConfig.to_config x l r) -[ tm ]->> (N.to_nat n) / (BoundedConfig.to_config x' l r)
+| inr _ => True
+end.
+Proof.
+  unfold BoundedConfig.multistep.
+  rewrite N_iter_until_spec'.
+  induction n using N.peano_ind; cbn; intros.
+  - constructor.
+  - rewrite N.iter_succ.
+    destruct (N.iter n (f_if_inl (BoundedConfig.step1 tm)) (inl x)); trivial.
+    unfold f_if_inl.
+    unfold BoundedConfig.step1.
+    destruct_spec (BoundedConfig_step_spec); trivial.
+    destruct p as [x' _].
+    intros.
+    replace (N.to_nat (N.succ n)) with ((N.to_nat n)+1) by lia.
+    eapply multistep_trans; eauto.
+Qed.
+
+Lemma BoundedConfig_progress_spec x n:
+match BoundedConfig.progress tm x n with
+| inl x' =>
+    forall l r,
+    (BoundedConfig.to_config x l r) -[ tm ]->+ (BoundedConfig.to_config x' l r)
+| inr _ => True
+end.
+Proof.
+  destruct n as [|n].
+  1: cbn; trivial.
+  unfold BoundedConfig.progress.
+  destruct_spec (BoundedConfig_multistep_spec); trivial.
+  intros.
+  eapply multistep_progress.
+  applys_eq H.
+  replace (N.to_nat (N.pos n)) with (S ((N.to_nat (N.pos n))-1)) by lia.
+  reflexivity.
+Qed.
+
+
+Inductive TC_state_WF:TC_state.T->nat->Prop :=
+| TC_state_WF_intro bc t0 h0 hs n:
+    c0 -[ tm ]->> n / (BoundedConfig.to_config bc (const s0) (const s0)) ->
+    TC_state_WF (TC_state.Build_T bc t0 h0 hs) n.
+
+Lemma TC_state_upd_spec x n:
+  TC_state_WF x n ->
+  match TC_state.upd tm x with
+  | inl x' =>
+    exists n', TC_state_WF x' n' /\ n'<=S n
+  | inr (x',h) => halts_at tm c0 n h
+  end.
+Proof.
+  destruct x as [bc t0 h0 hs]; cbn; intros.
+  inverts H.
+  destruct_spec (BoundedConfig_step_spec); trivial.
+  - destruct p as [x' h].
+    exists (S n).
+    split. 2: lia.
+    econstructor.
+    replace (S n) with (n+1) by lia.
+    eapply multistep_trans; eauto.
+  - destruct bc as [l r s sgn].
+    destruct r as [|m r].
+    + exists n.
+      split. 2: lia.
+      econstructor.
+      apply H5.
+    + cbn in H.
+      destruct H as [H|H]; try congruence.
+      destruct sgn; econstructor; eauto; apply H.
+Qed.
+
+Lemma TC_state_upds_spec x n m:
+  TC_state_WF x n ->
+  match TC_state.upds tm x m with
+  | inl x' =>
+    exists n', TC_state_WF x' n' /\ n'<=n+(N.to_nat m)
+  | inr (x',h) =>
+    exists n', halts_at tm c0 n' h /\ n'<=n+(N.to_nat m)
+  end.
+Proof.
+  intros H.
+  unfold TC_state.upds.
+  rewrite N_iter_until_spec'.
+  induction m using N.peano_ind.
+  - cbn.
+    exists n.
+    split; auto; lia.
+  - rewrite N.iter_succ.
+    destruct (N.iter m (f_if_inl (TC_state.upd tm)) (inl x)) eqn:E.
+    + destruct IHm as [n' [Hm1 Hm2]].
+      cbn.
+      destruct_spec TC_state_upd_spec.
+      * specialize (H0 _ Hm1).
+        destruct H0 as [n'0 [Hm3 Hm4]].
+        exists n'0.
+        split; auto; lia.
+      * destruct p as [x0 h].
+        eexists; split; eauto; lia.
+    + cbn.
+      destruct p as [x0 h].
+      destruct IHm as [n' [Hm1 Hm2]].
+      eexists; split; eauto; lia.
+Qed.
+
+Fixpoint N_list_sum (ls:list N):N :=
+match ls with
+| nil => N0
+| h::t => (h+(N_list_sum t))%N
+end.
+
+Lemma repeat_s0_const_s0 n:
+  repeat s0 n *> const s0 = const s0.
+Proof.
+  induction n.
+  1: reflexivity.
+  cbn.
+  rewrite IHn.
+  rewrite <-const_unfold.
+  reflexivity.
+Qed.
+
+
+Lemma TC_state_check_TC_spec t n:
+  TC_state_WF t n ->
+  if TC_state.check_TC tm t then ~halts tm c0 else True.
+Proof.
+  intros H.
+  inverts H.
+  unfold TC_state.check_TC.
+  cbn[TC_state.hs].
+  cbn[TC_state.bc].
+  destruct (TC_state.check_TC_2 hs) as [[p d]|]; trivial.
+  destruct (snd (BoundedConfig.steps' tm bc (to_N (p)))) as [[[ld1 rd1] _] _].
+  destruct bc as [l r s sgn].
+  destruct hs as [|[[_ sgn0] _]]; trivial.
+  destruct (eqb sgn sgn0).
+  - destruct_spec (BoundedConfig_progress_spec); trivial.
+    destruct t as [l2 r2 s2 sgn2].
+    destruct (eqb_spec s2 s); trivial.
+    destruct (eqb_spec sgn2 sgn); trivial.
+    destruct (eqb_spec r2 r); trivial.
+    remember (firstn ld1 l) as l1.
+    remember (skipn (length l1) l2) as l3.
+    destruct (eqb_spec l2 (l1++l3)); trivial.
+    subst s2 sgn2 r2.
+    cbn in H0,H.
+    rewrite e2 in H.
+    destruct sgn.
+    + eapply multistep_nonhalt.
+      1: eapply without_counter,H0.
+      rewrite <-(firstn_skipn ld1 l).
+      rewrite <-Heql1.
+      repeat rewrite Str_app_assoc.
+      eapply progress_nonhalt_simple with (C:=fun t => const s0 <* r <{{s}} l1 *> t).
+      intros t.
+      eexists.
+      specialize (H (const s0) t).
+      repeat rewrite Str_app_assoc in H.
+      rewrite repeat_s0_const_s0 in H.
+      apply H.
+    + eapply multistep_nonhalt.
+      1: eapply without_counter,H0.
+      rewrite <-(firstn_skipn ld1 l).
+      rewrite <-Heql1.
+      repeat rewrite Str_app_assoc.
+      eapply progress_nonhalt_simple with (C:=fun t => t <* l1 {{s}}> r *> const s0).
+      intros t.
+      eexists.
+      specialize (H t (const s0)).
+      repeat rewrite Str_app_assoc in H.
+      rewrite repeat_s0_const_s0 in H.
+      apply H.
+  - destruct_spec (BoundedConfig_progress_spec); trivial.
+    destruct t as [l2 r2 s2 sgn2].
+    destruct (eqb_spec s2 s); trivial.
+    destruct (eqb_spec sgn2 sgn); trivial.
+    destruct (eqb_spec l2 l); trivial.
+    remember (firstn rd1 r) as r1.
+    remember (skipn (length r1) r2) as r3.
+    destruct (eqb_spec r2 (r1++r3)); trivial.
+    subst s2 sgn2 l2.
+    cbn in H0,H.
+    rewrite e2 in H.
+    destruct sgn.
+    + eapply multistep_nonhalt.
+      1: eapply without_counter,H0.
+      rewrite <-(firstn_skipn rd1 r).
+      rewrite <-Heqr1.
+      repeat rewrite Str_app_assoc.
+      eapply progress_nonhalt_simple with (C:=fun t => t <* r1 <{{s}} l *> const s0).
+      intros t.
+      eexists.
+      specialize (H t (const s0)).
+      repeat rewrite Str_app_assoc in H.
+      rewrite repeat_s0_const_s0 in H.
+      apply H.
+    + eapply multistep_nonhalt.
+      1: eapply without_counter,H0.
+      rewrite <-(firstn_skipn rd1 r).
+      rewrite <-Heqr1.
+      repeat rewrite Str_app_assoc.
+      eapply progress_nonhalt_simple with (C:=fun t => const s0 <* l {{s}}> r1 *> t).
+      intros t.
+      eexists.
+      specialize (H (const s0) t).
+      repeat rewrite Str_app_assoc in H.
+      rewrite repeat_s0_const_s0 in H.
+      apply H.
+Qed.
+
+Lemma TC_state_decide_0_spec x n ls:
+  TC_state_WF x n ->
+  match (TC_state.decide_0 tm ls x) with
+  | (Halt h,_) => exists n', halts_at tm c0 n' h /\ n'<=n+(N.to_nat (N_list_sum ls))
+  | (NonHalt,_) => ~halts tm c0
+  | (Unknown,x') => exists n', TC_state_WF x' n' /\ n'<=n+(N.to_nat (N_list_sum ls))
+  end.
+Proof.
+  gen x n.
+  induction ls; intros.
+  1: cbn; exists n; split; auto; lia.
+  cbn.
+  pose proof (TC_state_upds_spec x _ a H).
+  destruct (TC_state.upds tm x a).
+  - destruct_spec (TC_state_check_TC_spec).
+    + destruct H0 as [n' [Hm1 Hm2]]. 
+      eauto.
+    + destruct H0 as [n' [Hm1 Hm2]].
+      specialize (IHls _ _ Hm1).
+      destruct_spec TC_state.decide_0.
+      destruct d.
+      * destruct IHls as [n'0 [Hm3 Hm4]].
+        exists n'0.
+        split; auto; lia.
+      * apply IHls.
+      * destruct IHls as [n'0 [Hm3 Hm4]].
+        exists n'0.
+        split; auto; lia.
+  - destruct p as [x' h].
+    destruct H0 as [n' [Hm1 Hm2]].
+    exists n'.
+    split; auto; lia.
+Qed.
+
+
+Lemma BoundedConfig_step_d_spec x d:
+match BoundedConfig.step_d tm (x,d) with
+| Some (x',d') =>
+    forall l r,
+    (BoundedConfig.to_config x l r) -[ tm ]-> (BoundedConfig.to_config x' l r)
+| None => True
+end.
+Proof.
+  destruct x as [l [|m r] s sgn]; cbn; trivial.
+  destruct (tm (s,m)) as [[[m' sgn'] s']|] eqn:E; trivial.
+  destruct sgn,sgn'; cbn; intros; constructor; apply E.
+Qed.
+
+Lemma find_cycle_0_spec x0 x1 d n:
+if BoundedConfig.find_cycle_0 tm x0 (x1,d) n then
+  (forall l r,
+  (BoundedConfig.to_config x0 l r) -[ tm ]->* (BoundedConfig.to_config x1 l r)) ->
+  forall l r,
+  ~halts tm (BoundedConfig.to_config x0 l r)
+else True.
+Proof.
+  Import BoundedConfig.
+  gen x1 d.
+  induction n; intros.
+  1: cbn; trivial.
+  cbn[BoundedConfig.find_cycle_0].
+  pose proof (BoundedConfig_step_d_spec x1 d).
+  destruct (BoundedConfig.step_d tm (x1, d)); trivial.
+  destruct p as [x2a x2b].
+  destruct (eqb x2b uint_0 && eqb x0 x2a)%bool eqn:E.
+  - destruct (eqb_spec x2b uint_0).
+    2: cbn in E; congruence.
+    destruct (eqb_spec x0 x2a).
+    2: congruence.
+    intros H0 l r.
+    eapply progress_nonhalt_simple with (C:=fun _:unit=>(to_config x0 l r)).
+    1: apply tt.
+    intros _.
+    exists tt.
+    subst x2a.
+    eapply evstep_progress_trans; eauto.
+  - specialize (IHn x2a x2b).
+    destruct_spec find_cycle_0; trivial.
+    intros H1.
+    apply IHn.
+    intros l r.
+    eapply progress_evstep.
+    eapply evstep_progress_trans; eauto.
+Qed.
+
+Lemma find_cycle_spec x0 n:
+if BoundedConfig.find_cycle tm x0 n then
+  forall l r,
+  ~halts tm (BoundedConfig.to_config x0 l r)
+else True.
+Proof.
+  unfold find_cycle.
+  pose proof (find_cycle_0_spec x0 x0 uint_0 n) as H.
+  destruct (find_cycle_0 tm x0 (x0, uint_0) n); trivial.
+  intros.
+  apply H.
+  intros.
+  auto.
+Qed.
+
+Lemma TC_state_decide_1_spec x n ls:
+  TC_state_WF x n ->
+  match (TC_state.decide_1 tm ls x) with
+  | (Halt h,_) => exists n', halts_at tm c0 n' h /\ n'<=n+(N.to_nat (N_list_sum (map N_list_sum (map fst ls))))
+  | (NonHalt,_) => ~halts tm c0
+  | (Unknown,x') => exists n', TC_state_WF x' n' /\ n'<=n+(N.to_nat (N_list_sum (map N_list_sum (map fst ls))))
+  end.
+Proof.
+  gen x n.
+  induction ls; intros.
+  1: cbn; exists n; split; auto; lia.
+  cbn.
+  destruct a as [n0 n1].
+  pose proof (TC_state_decide_0_spec x _ n0 H).
+  destruct (TC_state.decide_0 tm n0 x).
+  - cbn[fst].
+    destruct d.
+    + destruct H0 as [n' [Hm1 Hm2]]. 
+      exists n'.
+      split; auto; lia.
+    + apply H0.
+    + destruct_spec (find_cycle_spec).
+      * eapply multistep_nonhalt.
+        2: apply (H1 (const s0) (const s0)).
+        destruct H0 as [n' [Hm1 Hm2]]. 
+        inverts Hm1.
+        eapply without_counter; eauto.
+      * destruct H0 as [n' [Hm1 Hm2]]. 
+        specialize (IHls _ _ Hm1).
+        destruct_spec TC_state.decide_1.
+        destruct d.
+        -- destruct IHls as [n'0 [Hm3 Hm4]].
+           exists n'0. split; auto; lia.
+        -- apply IHls.
+        -- destruct IHls as [n'0 [Hm3 Hm4]].
+           exists n'0. split; auto; lia.
+Qed.
+
+Lemma TC_state_decide_spec ls:
+  match (TC_state.decide tm ls) with
+  | (Halt h,_) => exists n', halts_at tm c0 n' h /\ n'<=(N.to_nat (N_list_sum (map N_list_sum (map fst ls))))
+  | (NonHalt,_) => ~halts tm c0
+  | (Unknown,x') => exists n', TC_state_WF x' n' /\ n'<=(N.to_nat (N_list_sum (map N_list_sum (map fst ls))))
+  end.
+Proof.
+  unfold TC_state.decide.
+  apply (TC_state_decide_1_spec TC_state.T0 O ls).
+  constructor; auto.
+Qed.
+
+End tm_ctx.
+
+End TC.
+
+
